clean up my own case study and add to CI

case-studies/tapl-exercise/sysf.v
@@ -1,5 +1,11 @@
 Require Import core unscoped.
 
+Require Import core_axioms unscoped_axioms.
+Require Import Setoid Morphisms Relation_Definitions.
+
+
+Module Core.
+
 Inductive ty : Type :=
   | var_ty : nat -> ty
   | arr : ty -> ty -> ty
@@ -7,25 +13,19 @@ Inductive ty : Type :=
 
 Lemma congr_arr {s0 : ty} {s1 : ty} {t0 : ty} {t1 : ty} (H0 : s0 = t0)
   (H1 : s1 = t1) : arr s0 s1 = arr t0 t1.
-
 Proof.
 exact (eq_trans (eq_trans eq_refl (ap (fun x => arr x s1) H0))
-                (ap (fun x => arr t0 x) H1)).
-
+         (ap (fun x => arr t0 x) H1)).
 Qed.
 
 Lemma congr_all {s0 : ty} {t0 : ty} (H0 : s0 = t0) : all s0 = all t0.
-
 Proof.
 exact (eq_trans eq_refl (ap (fun x => all x) H0)).
-
 Qed.
 
 Lemma upRen_ty_ty (xi : nat -> nat) : nat -> nat.
-
 Proof.
 exact (up_ren xi).
-
 Defined.
 
 Fixpoint ren_ty (xi_ty : nat -> nat) (s : ty) {struct s} : ty :=
@@ -36,10 +36,8 @@ Fixpoint ren_ty (xi_ty : nat -> nat) (s : ty) {struct s} : ty :=
   end.
 
 Lemma up_ty_ty (sigma : nat -> ty) : nat -> ty.
-
 Proof.
 exact (scons (var_ty var_zero) (funcomp (ren_ty shift) sigma)).
-
 Defined.
 
 Fixpoint subst_ty (sigma_ty : nat -> ty) (s : ty) {struct s} : ty :=
@@ -51,14 +49,12 @@ Fixpoint subst_ty (sigma_ty : nat -> ty) (s : ty) {struct s} : ty :=
 
 Lemma upId_ty_ty (sigma : nat -> ty) (Eq : forall x, sigma x = var_ty x) :
   forall x, up_ty_ty sigma x = var_ty x.
-
 Proof.
 exact (fun n =>
-              match n with
-              | S n' => ap (ren_ty shift) (Eq n')
-              | O => eq_refl
-              end).
-
+       match n with
+       | S n' => ap (ren_ty shift) (Eq n')
+       | O => eq_refl
+       end).
 Qed.
 
 Fixpoint idSubst_ty (sigma_ty : nat -> ty)
@@ -75,21 +71,18 @@ subst_ty sigma_ty s = s :=
 Lemma upExtRen_ty_ty (xi : nat -> nat) (zeta : nat -> nat)
   (Eq : forall x, xi x = zeta x) :
   forall x, upRen_ty_ty xi x = upRen_ty_ty zeta x.
-
 Proof.
-exact (fun n =>
-              match n with
-              | S n' => ap shift (Eq n')
-              | O => eq_refl
-              end).
-
+exact (fun n => match n with
+                | S n' => ap shift (Eq n')
+                | O => eq_refl
+                end).
 Qed.
 
 Fixpoint extRen_ty (xi_ty : nat -> nat) (zeta_ty : nat -> nat)
 (Eq_ty : forall x, xi_ty x = zeta_ty x) (s : ty) {struct s} :
 ren_ty xi_ty s = ren_ty zeta_ty s :=
   match s with
-  | var_ty s0 => ap var_ty (Eq_ty s0)
+  | var_ty s0 => ap (var_ty) (Eq_ty s0)
   | arr s0 s1 =>
       congr_arr (extRen_ty xi_ty zeta_ty Eq_ty s0)
         (extRen_ty xi_ty zeta_ty Eq_ty s1)
@@ -102,14 +95,12 @@ ren_ty xi_ty s = ren_ty zeta_ty s :=
 Lemma upExt_ty_ty (sigma : nat -> ty) (tau : nat -> ty)
   (Eq : forall x, sigma x = tau x) :
   forall x, up_ty_ty sigma x = up_ty_ty tau x.
-
 Proof.
 exact (fun n =>
-              match n with
-              | S n' => ap (ren_ty shift) (Eq n')
-              | O => eq_refl
-              end).
-
+       match n with
+       | S n' => ap (ren_ty shift) (Eq n')
+       | O => eq_refl
+       end).
 Qed.
 
 Fixpoint ext_ty (sigma_ty : nat -> ty) (tau_ty : nat -> ty)
@@ -129,17 +120,15 @@ subst_ty sigma_ty s = subst_ty tau_ty s :=
 Lemma up_ren_ren_ty_ty (xi : nat -> nat) (zeta : nat -> nat)
   (rho : nat -> nat) (Eq : forall x, funcomp zeta xi x = rho x) :
   forall x, funcomp (upRen_ty_ty zeta) (upRen_ty_ty xi) x = upRen_ty_ty rho x.
-
 Proof.
 exact (up_ren_ren xi zeta rho Eq).
-
 Qed.
 
 Fixpoint compRenRen_ty (xi_ty : nat -> nat) (zeta_ty : nat -> nat)
 (rho_ty : nat -> nat) (Eq_ty : forall x, funcomp zeta_ty xi_ty x = rho_ty x)
 (s : ty) {struct s} : ren_ty zeta_ty (ren_ty xi_ty s) = ren_ty rho_ty s :=
   match s with
-  | var_ty s0 => ap var_ty (Eq_ty s0)
+  | var_ty s0 => ap (var_ty) (Eq_ty s0)
   | arr s0 s1 =>
       congr_arr (compRenRen_ty xi_ty zeta_ty rho_ty Eq_ty s0)
         (compRenRen_ty xi_ty zeta_ty rho_ty Eq_ty s1)
@@ -152,14 +141,12 @@ Fixpoint compRenRen_ty (xi_ty : nat -> nat) (zeta_ty : nat -> nat)
 Lemma up_ren_subst_ty_ty (xi : nat -> nat) (tau : nat -> ty)
   (theta : nat -> ty) (Eq : forall x, funcomp tau xi x = theta x) :
   forall x, funcomp (up_ty_ty tau) (upRen_ty_ty xi) x = up_ty_ty theta x.
-
 Proof.
 exact (fun n =>
-              match n with
-              | S n' => ap (ren_ty shift) (Eq n')
-              | O => eq_refl
-              end).
-
+       match n with
+       | S n' => ap (ren_ty shift) (Eq n')
+       | O => eq_refl
+       end).
 Qed.
 
 Fixpoint compRenSubst_ty (xi_ty : nat -> nat) (tau_ty : nat -> ty)
@@ -183,22 +170,20 @@ Lemma up_subst_ren_ty_ty (sigma : nat -> ty) (zeta_ty : nat -> nat)
   forall x,
   funcomp (ren_ty (upRen_ty_ty zeta_ty)) (up_ty_ty sigma) x =
   up_ty_ty theta x.
-
 Proof.
 exact (fun n =>
-              match n with
-              | S n' =>
-                  eq_trans
-                    (compRenRen_ty shift (upRen_ty_ty zeta_ty)
-                       (funcomp shift zeta_ty) (fun x => eq_refl) (sigma n'))
-                    (eq_trans
-                       (eq_sym
-                          (compRenRen_ty zeta_ty shift
-                             (funcomp shift zeta_ty) (fun x => eq_refl)
-                             (sigma n'))) (ap (ren_ty shift) (Eq n')))
-              | O => eq_refl
-              end).
-
+       match n with
+       | S n' =>
+           eq_trans
+             (compRenRen_ty shift (upRen_ty_ty zeta_ty)
+                (funcomp shift zeta_ty) (fun x => eq_refl) (sigma n'))
+             (eq_trans
+                (eq_sym
+                   (compRenRen_ty zeta_ty shift (funcomp shift zeta_ty)
+                      (fun x => eq_refl) (sigma n')))
+                (ap (ren_ty shift) (Eq n')))
+       | O => eq_refl
+       end).
 Qed.
 
 Fixpoint compSubstRen_ty (sigma_ty : nat -> ty) (zeta_ty : nat -> nat)
@@ -222,24 +207,21 @@ Lemma up_subst_subst_ty_ty (sigma : nat -> ty) (tau_ty : nat -> ty)
   (Eq : forall x, funcomp (subst_ty tau_ty) sigma x = theta x) :
   forall x,
   funcomp (subst_ty (up_ty_ty tau_ty)) (up_ty_ty sigma) x = up_ty_ty theta x.
-
 Proof.
 exact (fun n =>
-              match n with
-              | S n' =>
-                  eq_trans
-                    (compRenSubst_ty shift (up_ty_ty tau_ty)
-                       (funcomp (up_ty_ty tau_ty) shift) (fun x => eq_refl)
-                       (sigma n'))
-                    (eq_trans
-                       (eq_sym
-                          (compSubstRen_ty tau_ty shift
-                             (funcomp (ren_ty shift) tau_ty)
-                             (fun x => eq_refl) (sigma n')))
-                       (ap (ren_ty shift) (Eq n')))
-              | O => eq_refl
-              end).
-
+       match n with
+       | S n' =>
+           eq_trans
+             (compRenSubst_ty shift (up_ty_ty tau_ty)
+                (funcomp (up_ty_ty tau_ty) shift) (fun x => eq_refl)
+                (sigma n'))
+             (eq_trans
+                (eq_sym
+                   (compSubstRen_ty tau_ty shift
+                      (funcomp (ren_ty shift) tau_ty) (fun x => eq_refl)
+                      (sigma n'))) (ap (ren_ty shift) (Eq n')))
+       | O => eq_refl
+       end).
 Qed.
 
 Fixpoint compSubstSubst_ty (sigma_ty : nat -> ty) (tau_ty : nat -> ty)
@@ -259,21 +241,19 @@ subst_ty tau_ty (subst_ty sigma_ty s) = subst_ty theta_ty s :=
   end.
 
 Lemma rinstInst_up_ty_ty (xi : nat -> nat) (sigma : nat -> ty)
-  (Eq : forall x, funcomp var_ty xi x = sigma x) :
-  forall x, funcomp var_ty (upRen_ty_ty xi) x = up_ty_ty sigma x.
-
+  (Eq : forall x, funcomp (var_ty) xi x = sigma x) :
+  forall x, funcomp (var_ty) (upRen_ty_ty xi) x = up_ty_ty sigma x.
 Proof.
 exact (fun n =>
-              match n with
-              | S n' => ap (ren_ty shift) (Eq n')
-              | O => eq_refl
-              end).
-
+       match n with
+       | S n' => ap (ren_ty shift) (Eq n')
+       | O => eq_refl
+       end).
 Qed.
 
 Fixpoint rinst_inst_ty (xi_ty : nat -> nat) (sigma_ty : nat -> ty)
-(Eq_ty : forall x, funcomp var_ty xi_ty x = sigma_ty x) (s : ty) {struct s} :
-ren_ty xi_ty s = subst_ty sigma_ty s :=
+(Eq_ty : forall x, funcomp (var_ty) xi_ty x = sigma_ty x) (s : ty) {struct s}
+   : ren_ty xi_ty s = subst_ty sigma_ty s :=
   match s with
   | var_ty s0 => Eq_ty s0
   | arr s0 s1 =>
@@ -287,36 +267,113 @@ ren_ty xi_ty s = subst_ty sigma_ty s :=
 
 Lemma renRen_ty (xi_ty : nat -> nat) (zeta_ty : nat -> nat) (s : ty) :
   ren_ty zeta_ty (ren_ty xi_ty s) = ren_ty (funcomp zeta_ty xi_ty) s.
-
 Proof.
 exact (compRenRen_ty xi_ty zeta_ty _ (fun n => eq_refl) s).
-
 Qed.
 
-Lemma compRen_ty (sigma_ty : nat -> ty) (zeta_ty : nat -> nat) (s : ty) :
+Lemma renRen'_ty_pointwise (xi_ty : nat -> nat) (zeta_ty : nat -> nat) :
+  pointwise_relation _ eq (funcomp (ren_ty zeta_ty) (ren_ty xi_ty))
+    (ren_ty (funcomp zeta_ty xi_ty)).
+Proof.
+exact (fun s => compRenRen_ty xi_ty zeta_ty _ (fun n => eq_refl) s).
+Qed.
+
+Lemma substRen_ty (sigma_ty : nat -> ty) (zeta_ty : nat -> nat) (s : ty) :
   ren_ty zeta_ty (subst_ty sigma_ty s) =
   subst_ty (funcomp (ren_ty zeta_ty) sigma_ty) s.
-
 Proof.
 exact (compSubstRen_ty sigma_ty zeta_ty _ (fun n => eq_refl) s).
-
 Qed.
 
-Lemma renComp_ty (xi_ty : nat -> nat) (tau_ty : nat -> ty) (s : ty) :
-  subst_ty tau_ty (ren_ty xi_ty s) = subst_ty (funcomp tau_ty xi_ty) s.
+Lemma substRen_ty_pointwise (sigma_ty : nat -> ty) (zeta_ty : nat -> nat) :
+  pointwise_relation _ eq (funcomp (ren_ty zeta_ty) (subst_ty sigma_ty))
+    (subst_ty (funcomp (ren_ty zeta_ty) sigma_ty)).
+Proof.
+exact (fun s => compSubstRen_ty sigma_ty zeta_ty _ (fun n => eq_refl) s).
+Qed.
 
+Lemma renSubst_ty (xi_ty : nat -> nat) (tau_ty : nat -> ty) (s : ty) :
+  subst_ty tau_ty (ren_ty xi_ty s) = subst_ty (funcomp tau_ty xi_ty) s.
 Proof.
 exact (compRenSubst_ty xi_ty tau_ty _ (fun n => eq_refl) s).
-
 Qed.
 
-Lemma compComp_ty (sigma_ty : nat -> ty) (tau_ty : nat -> ty) (s : ty) :
+Lemma renSubst_ty_pointwise (xi_ty : nat -> nat) (tau_ty : nat -> ty) :
+  pointwise_relation _ eq (funcomp (subst_ty tau_ty) (ren_ty xi_ty))
+    (subst_ty (funcomp tau_ty xi_ty)).
+Proof.
+exact (fun s => compRenSubst_ty xi_ty tau_ty _ (fun n => eq_refl) s).
+Qed.
+
+Lemma substSubst_ty (sigma_ty : nat -> ty) (tau_ty : nat -> ty) (s : ty) :
   subst_ty tau_ty (subst_ty sigma_ty s) =
   subst_ty (funcomp (subst_ty tau_ty) sigma_ty) s.
-
 Proof.
 exact (compSubstSubst_ty sigma_ty tau_ty _ (fun n => eq_refl) s).
+Qed.
 
+Lemma substSubst_ty_pointwise (sigma_ty : nat -> ty) (tau_ty : nat -> ty) :
+  pointwise_relation _ eq (funcomp (subst_ty tau_ty) (subst_ty sigma_ty))
+    (subst_ty (funcomp (subst_ty tau_ty) sigma_ty)).
+Proof.
+exact (fun s => compSubstSubst_ty sigma_ty tau_ty _ (fun n => eq_refl) s).
+Qed.
+
+Lemma rinstInst'_ty (xi_ty : nat -> nat) (s : ty) :
+  ren_ty xi_ty s = subst_ty (funcomp (var_ty) xi_ty) s.
+Proof.
+exact (rinst_inst_ty xi_ty _ (fun n => eq_refl) s).
+Qed.
+
+Lemma rinstInst'_ty_pointwise (xi_ty : nat -> nat) :
+  pointwise_relation _ eq (ren_ty xi_ty) (subst_ty (funcomp (var_ty) xi_ty)).
+Proof.
+exact (fun s => rinst_inst_ty xi_ty _ (fun n => eq_refl) s).
+Qed.
+
+Lemma instId'_ty (s : ty) : subst_ty (var_ty) s = s.
+Proof.
+exact (idSubst_ty (var_ty) (fun n => eq_refl) s).
+Qed.
+
+Lemma instId'_ty_pointwise : pointwise_relation _ eq (subst_ty (var_ty)) id.
+Proof.
+exact (fun s => idSubst_ty (var_ty) (fun n => eq_refl) s).
+Qed.
+
+Lemma rinstId'_ty (s : ty) : ren_ty id s = s.
+Proof.
+exact (eq_ind_r (fun t => t = s) (instId'_ty s) (rinstInst'_ty id s)).
+Qed.
+
+Lemma rinstId'_ty_pointwise : pointwise_relation _ eq (@ren_ty id) id.
+Proof.
+exact (fun s => eq_ind_r (fun t => t = s) (instId'_ty s) (rinstInst'_ty id s)).
+Qed.
+
+Lemma varL'_ty (sigma_ty : nat -> ty) (x : nat) :
+  subst_ty sigma_ty (var_ty x) = sigma_ty x.
+Proof.
+exact (eq_refl).
+Qed.
+
+Lemma varL'_ty_pointwise (sigma_ty : nat -> ty) :
+  pointwise_relation _ eq (funcomp (subst_ty sigma_ty) (var_ty)) sigma_ty.
+Proof.
+exact (fun x => eq_refl).
+Qed.
+
+Lemma varLRen'_ty (xi_ty : nat -> nat) (x : nat) :
+  ren_ty xi_ty (var_ty x) = var_ty (xi_ty x).
+Proof.
+exact (eq_refl).
+Qed.
+
+Lemma varLRen'_ty_pointwise (xi_ty : nat -> nat) :
+  pointwise_relation _ eq (funcomp (ren_ty xi_ty) (var_ty))
+    (funcomp (var_ty) xi_ty).
+Proof.
+exact (fun x => eq_refl).
 Qed.
 
 Inductive tm : Type :=
@@ -328,57 +385,43 @@ Inductive tm : Type :=
 
 Lemma congr_app {s0 : tm} {s1 : tm} {t0 : tm} {t1 : tm} (H0 : s0 = t0)
   (H1 : s1 = t1) : app s0 s1 = app t0 t1.
-
 Proof.
 exact (eq_trans (eq_trans eq_refl (ap (fun x => app x s1) H0))
-                (ap (fun x => app t0 x) H1)).
-
+         (ap (fun x => app t0 x) H1)).
 Qed.
 
 Lemma congr_tapp {s0 : tm} {s1 : ty} {t0 : tm} {t1 : ty} (H0 : s0 = t0)
   (H1 : s1 = t1) : tapp s0 s1 = tapp t0 t1.
-
 Proof.
 exact (eq_trans (eq_trans eq_refl (ap (fun x => tapp x s1) H0))
-                (ap (fun x => tapp t0 x) H1)).
-
+         (ap (fun x => tapp t0 x) H1)).
 Qed.
 
 Lemma congr_lam {s0 : ty} {s1 : tm} {t0 : ty} {t1 : tm} (H0 : s0 = t0)
   (H1 : s1 = t1) : lam s0 s1 = lam t0 t1.
-
 Proof.
 exact (eq_trans (eq_trans eq_refl (ap (fun x => lam x s1) H0))
-                (ap (fun x => lam t0 x) H1)).
-
+         (ap (fun x => lam t0 x) H1)).
 Qed.
 
 Lemma congr_tlam {s0 : tm} {t0 : tm} (H0 : s0 = t0) : tlam s0 = tlam t0.
-
 Proof.
 exact (eq_trans eq_refl (ap (fun x => tlam x) H0)).
-
 Qed.
 
 Lemma upRen_ty_tm (xi : nat -> nat) : nat -> nat.
-
 Proof.
 exact (xi).
-
 Defined.
 
 Lemma upRen_tm_ty (xi : nat -> nat) : nat -> nat.
-
 Proof.
 exact (xi).
-
 Defined.
 
 Lemma upRen_tm_tm (xi : nat -> nat) : nat -> nat.
-
 Proof.
 exact (up_ren xi).
-
 Defined.
 
 Fixpoint ren_tm (xi_ty : nat -> nat) (xi_tm : nat -> nat) (s : tm) {struct s}
@@ -394,24 +437,18 @@ Fixpoint ren_tm (xi_ty : nat -> nat) (xi_tm : nat -> nat) (s : tm) {struct s}
   end.
 
 Lemma up_ty_tm (sigma : nat -> tm) : nat -> tm.
-
 Proof.
 exact (funcomp (ren_tm shift id) sigma).
-
 Defined.
 
 Lemma up_tm_ty (sigma : nat -> ty) : nat -> ty.
-
 Proof.
 exact (funcomp (ren_ty id) sigma).
-
 Defined.
 
 Lemma up_tm_tm (sigma : nat -> tm) : nat -> tm.
-
 Proof.
 exact (scons (var_tm var_zero) (funcomp (ren_tm id shift) sigma)).
-
 Defined.
 
 Fixpoint subst_tm (sigma_ty : nat -> ty) (sigma_tm : nat -> tm) (s : tm)
@@ -429,30 +466,24 @@ Fixpoint subst_tm (sigma_ty : nat -> ty) (sigma_tm : nat -> tm) (s : tm)
 
 Lemma upId_ty_tm (sigma : nat -> tm) (Eq : forall x, sigma x = var_tm x) :
   forall x, up_ty_tm sigma x = var_tm x.
-
 Proof.
 exact (fun n => ap (ren_tm shift id) (Eq n)).
-
 Qed.
 
 Lemma upId_tm_ty (sigma : nat -> ty) (Eq : forall x, sigma x = var_ty x) :
   forall x, up_tm_ty sigma x = var_ty x.
-
 Proof.
 exact (fun n => ap (ren_ty id) (Eq n)).
-
 Qed.
 
 Lemma upId_tm_tm (sigma : nat -> tm) (Eq : forall x, sigma x = var_tm x) :
   forall x, up_tm_tm sigma x = var_tm x.
-
 Proof.
 exact (fun n =>
-              match n with
-              | S n' => ap (ren_tm id shift) (Eq n')
-              | O => eq_refl
-              end).
-
+       match n with
+       | S n' => ap (ren_tm id shift) (Eq n')
+       | O => eq_refl
+       end).
 Qed.
 
 Fixpoint idSubst_tm (sigma_ty : nat -> ty) (sigma_tm : nat -> tm)
@@ -480,32 +511,25 @@ subst_tm sigma_ty sigma_tm s = s :=
 Lemma upExtRen_ty_tm (xi : nat -> nat) (zeta : nat -> nat)
   (Eq : forall x, xi x = zeta x) :
   forall x, upRen_ty_tm xi x = upRen_ty_tm zeta x.
-
 Proof.
 exact (fun n => Eq n).
-
 Qed.
 
 Lemma upExtRen_tm_ty (xi : nat -> nat) (zeta : nat -> nat)
   (Eq : forall x, xi x = zeta x) :
   forall x, upRen_tm_ty xi x = upRen_tm_ty zeta x.
-
 Proof.
 exact (fun n => Eq n).
-
 Qed.
 
 Lemma upExtRen_tm_tm (xi : nat -> nat) (zeta : nat -> nat)
   (Eq : forall x, xi x = zeta x) :
   forall x, upRen_tm_tm xi x = upRen_tm_tm zeta x.
-
 Proof.
-exact (fun n =>
-              match n with
-              | S n' => ap shift (Eq n')
-              | O => eq_refl
-              end).
-
+exact (fun n => match n with
+                | S n' => ap shift (Eq n')
+                | O => eq_refl
+                end).
 Qed.
 
 Fixpoint extRen_tm (xi_ty : nat -> nat) (xi_tm : nat -> nat)
@@ -514,7 +538,7 @@ Fixpoint extRen_tm (xi_ty : nat -> nat) (xi_tm : nat -> nat)
 (Eq_tm : forall x, xi_tm x = zeta_tm x) (s : tm) {struct s} :
 ren_tm xi_ty xi_tm s = ren_tm zeta_ty zeta_tm s :=
   match s with
-  | var_tm s0 => ap var_tm (Eq_tm s0)
+  | var_tm s0 => ap (var_tm) (Eq_tm s0)
   | app s0 s1 =>
       congr_app (extRen_tm xi_ty xi_tm zeta_ty zeta_tm Eq_ty Eq_tm s0)
         (extRen_tm xi_ty xi_tm zeta_ty zeta_tm Eq_ty Eq_tm s1)
@@ -536,32 +560,26 @@ ren_tm xi_ty xi_tm s = ren_tm zeta_ty zeta_tm s :=
 Lemma upExt_ty_tm (sigma : nat -> tm) (tau : nat -> tm)
   (Eq : forall x, sigma x = tau x) :
   forall x, up_ty_tm sigma x = up_ty_tm tau x.
-
 Proof.
 exact (fun n => ap (ren_tm shift id) (Eq n)).
-
 Qed.
 
 Lemma upExt_tm_ty (sigma : nat -> ty) (tau : nat -> ty)
   (Eq : forall x, sigma x = tau x) :
   forall x, up_tm_ty sigma x = up_tm_ty tau x.
-
 Proof.
 exact (fun n => ap (ren_ty id) (Eq n)).
-
 Qed.
 
 Lemma upExt_tm_tm (sigma : nat -> tm) (tau : nat -> tm)
   (Eq : forall x, sigma x = tau x) :
   forall x, up_tm_tm sigma x = up_tm_tm tau x.
-
 Proof.
 exact (fun n =>
-              match n with
-              | S n' => ap (ren_tm id shift) (Eq n')
-              | O => eq_refl
-              end).
-
+       match n with
+       | S n' => ap (ren_tm id shift) (Eq n')
+       | O => eq_refl
+       end).
 Qed.
 
 Fixpoint ext_tm (sigma_ty : nat -> ty) (sigma_tm : nat -> tm)
@@ -592,28 +610,22 @@ subst_tm sigma_ty sigma_tm s = subst_tm tau_ty tau_tm s :=
 Lemma up_ren_ren_ty_tm (xi : nat -> nat) (zeta : nat -> nat)
   (rho : nat -> nat) (Eq : forall x, funcomp zeta xi x = rho x) :
   forall x, funcomp (upRen_ty_tm zeta) (upRen_ty_tm xi) x = upRen_ty_tm rho x.
-
 Proof.
 exact (Eq).
-
 Qed.
 
 Lemma up_ren_ren_tm_ty (xi : nat -> nat) (zeta : nat -> nat)
   (rho : nat -> nat) (Eq : forall x, funcomp zeta xi x = rho x) :
   forall x, funcomp (upRen_tm_ty zeta) (upRen_tm_ty xi) x = upRen_tm_ty rho x.
-
 Proof.
 exact (Eq).
-
 Qed.
 
 Lemma up_ren_ren_tm_tm (xi : nat -> nat) (zeta : nat -> nat)
   (rho : nat -> nat) (Eq : forall x, funcomp zeta xi x = rho x) :
   forall x, funcomp (upRen_tm_tm zeta) (upRen_tm_tm xi) x = upRen_tm_tm rho x.
-
 Proof.
 exact (up_ren_ren xi zeta rho Eq).
-
 Qed.
 
 Fixpoint compRenRen_tm (xi_ty : nat -> nat) (xi_tm : nat -> nat)
@@ -622,7 +634,7 @@ Fixpoint compRenRen_tm (xi_ty : nat -> nat) (xi_tm : nat -> nat)
 (Eq_tm : forall x, funcomp zeta_tm xi_tm x = rho_tm x) (s : tm) {struct s} :
 ren_tm zeta_ty zeta_tm (ren_tm xi_ty xi_tm s) = ren_tm rho_ty rho_tm s :=
   match s with
-  | var_tm s0 => ap var_tm (Eq_tm s0)
+  | var_tm s0 => ap (var_tm) (Eq_tm s0)
   | app s0 s1 =>
       congr_app
         (compRenRen_tm xi_ty xi_tm zeta_ty zeta_tm rho_ty rho_tm Eq_ty Eq_tm
@@ -648,32 +660,26 @@ ren_tm zeta_ty zeta_tm (ren_tm xi_ty xi_tm s) = ren_tm rho_ty rho_tm s :=
 Lemma up_ren_subst_ty_tm (xi : nat -> nat) (tau : nat -> tm)
   (theta : nat -> tm) (Eq : forall x, funcomp tau xi x = theta x) :
   forall x, funcomp (up_ty_tm tau) (upRen_ty_tm xi) x = up_ty_tm theta x.
-
 Proof.
 exact (fun n => ap (ren_tm shift id) (Eq n)).
-
 Qed.
 
 Lemma up_ren_subst_tm_ty (xi : nat -> nat) (tau : nat -> ty)
   (theta : nat -> ty) (Eq : forall x, funcomp tau xi x = theta x) :
   forall x, funcomp (up_tm_ty tau) (upRen_tm_ty xi) x = up_tm_ty theta x.
-
 Proof.
 exact (fun n => ap (ren_ty id) (Eq n)).
-
 Qed.
 
 Lemma up_ren_subst_tm_tm (xi : nat -> nat) (tau : nat -> tm)
   (theta : nat -> tm) (Eq : forall x, funcomp tau xi x = theta x) :
   forall x, funcomp (up_tm_tm tau) (upRen_tm_tm xi) x = up_tm_tm theta x.
-
 Proof.
 exact (fun n =>
-              match n with
-              | S n' => ap (ren_tm id shift) (Eq n')
-              | O => eq_refl
-              end).
-
+       match n with
+       | S n' => ap (ren_tm id shift) (Eq n')
+       | O => eq_refl
+       end).
 Qed.
 
 Fixpoint compRenSubst_tm (xi_ty : nat -> nat) (xi_tm : nat -> nat)
@@ -715,21 +721,18 @@ Lemma up_subst_ren_ty_tm (sigma : nat -> tm) (zeta_ty : nat -> nat)
   forall x,
   funcomp (ren_tm (upRen_ty_ty zeta_ty) (upRen_ty_tm zeta_tm))
     (up_ty_tm sigma) x = up_ty_tm theta x.
-
 Proof.
 exact (fun n =>
-              eq_trans
-                (compRenRen_tm shift id (upRen_ty_ty zeta_ty)
-                   (upRen_ty_tm zeta_tm) (funcomp shift zeta_ty)
-                   (funcomp id zeta_tm) (fun x => eq_refl) (fun x => eq_refl)
-                   (sigma n))
-                (eq_trans
-                   (eq_sym
-                      (compRenRen_tm zeta_ty zeta_tm shift id
-                         (funcomp shift zeta_ty) (funcomp id zeta_tm)
-                         (fun x => eq_refl) (fun x => eq_refl) (sigma n)))
-                   (ap (ren_tm shift id) (Eq n)))).
-
+       eq_trans
+         (compRenRen_tm shift id (upRen_ty_ty zeta_ty) (upRen_ty_tm zeta_tm)
+            (funcomp shift zeta_ty) (funcomp id zeta_tm) (fun x => eq_refl)
+            (fun x => eq_refl) (sigma n))
+         (eq_trans
+            (eq_sym
+               (compRenRen_tm zeta_ty zeta_tm shift id
+                  (funcomp shift zeta_ty) (funcomp id zeta_tm)
+                  (fun x => eq_refl) (fun x => eq_refl) (sigma n)))
+            (ap (ren_tm shift id) (Eq n)))).
 Qed.
 
 Lemma up_subst_ren_tm_ty (sigma : nat -> ty) (zeta_ty : nat -> nat)
@@ -738,18 +741,15 @@ Lemma up_subst_ren_tm_ty (sigma : nat -> ty) (zeta_ty : nat -> nat)
   forall x,
   funcomp (ren_ty (upRen_tm_ty zeta_ty)) (up_tm_ty sigma) x =
   up_tm_ty theta x.
-
 Proof.
 exact (fun n =>
-              eq_trans
-                (compRenRen_ty id (upRen_tm_ty zeta_ty) (funcomp id zeta_ty)
-                   (fun x => eq_refl) (sigma n))
-                (eq_trans
-                   (eq_sym
-                      (compRenRen_ty zeta_ty id (funcomp id zeta_ty)
-                         (fun x => eq_refl) (sigma n)))
-                   (ap (ren_ty id) (Eq n)))).
-
+       eq_trans
+         (compRenRen_ty id (upRen_tm_ty zeta_ty) (funcomp id zeta_ty)
+            (fun x => eq_refl) (sigma n))
+         (eq_trans
+            (eq_sym
+               (compRenRen_ty zeta_ty id (funcomp id zeta_ty)
+                  (fun x => eq_refl) (sigma n))) (ap (ren_ty id) (Eq n)))).
 Qed.
 
 Lemma up_subst_ren_tm_tm (sigma : nat -> tm) (zeta_ty : nat -> nat)
@@ -758,25 +758,23 @@ Lemma up_subst_ren_tm_tm (sigma : nat -> tm) (zeta_ty : nat -> nat)
   forall x,
   funcomp (ren_tm (upRen_tm_ty zeta_ty) (upRen_tm_tm zeta_tm))
     (up_tm_tm sigma) x = up_tm_tm theta x.
-
 Proof.
 exact (fun n =>
-              match n with
-              | S n' =>
-                  eq_trans
-                    (compRenRen_tm id shift (upRen_tm_ty zeta_ty)
-                       (upRen_tm_tm zeta_tm) (funcomp id zeta_ty)
-                       (funcomp shift zeta_tm) (fun x => eq_refl)
-                       (fun x => eq_refl) (sigma n'))
-                    (eq_trans
-                       (eq_sym
-                          (compRenRen_tm zeta_ty zeta_tm id shift
-                             (funcomp id zeta_ty) (funcomp shift zeta_tm)
-                             (fun x => eq_refl) (fun x => eq_refl) (sigma n')))
-                       (ap (ren_tm id shift) (Eq n')))
-              | O => eq_refl
-              end).
-
+       match n with
+       | S n' =>
+           eq_trans
+             (compRenRen_tm id shift (upRen_tm_ty zeta_ty)
+                (upRen_tm_tm zeta_tm) (funcomp id zeta_ty)
+                (funcomp shift zeta_tm) (fun x => eq_refl) (fun x => eq_refl)
+                (sigma n'))
+             (eq_trans
+                (eq_sym
+                   (compRenRen_tm zeta_ty zeta_tm id shift
+                      (funcomp id zeta_ty) (funcomp shift zeta_tm)
+                      (fun x => eq_refl) (fun x => eq_refl) (sigma n')))
+                (ap (ren_tm id shift) (Eq n')))
+       | O => eq_refl
+       end).
 Qed.
 
 Fixpoint compSubstRen_tm (sigma_ty : nat -> ty) (sigma_tm : nat -> tm)
@@ -820,22 +818,19 @@ Lemma up_subst_subst_ty_tm (sigma : nat -> tm) (tau_ty : nat -> ty)
   forall x,
   funcomp (subst_tm (up_ty_ty tau_ty) (up_ty_tm tau_tm)) (up_ty_tm sigma) x =
   up_ty_tm theta x.
-
 Proof.
 exact (fun n =>
-              eq_trans
-                (compRenSubst_tm shift id (up_ty_ty tau_ty) (up_ty_tm tau_tm)
-                   (funcomp (up_ty_ty tau_ty) shift)
-                   (funcomp (up_ty_tm tau_tm) id) (fun x => eq_refl)
-                   (fun x => eq_refl) (sigma n))
-                (eq_trans
-                   (eq_sym
-                      (compSubstRen_tm tau_ty tau_tm shift id
-                         (funcomp (ren_ty shift) tau_ty)
-                         (funcomp (ren_tm shift id) tau_tm)
-                         (fun x => eq_refl) (fun x => eq_refl) (sigma n)))
-                   (ap (ren_tm shift id) (Eq n)))).
-
+       eq_trans
+         (compRenSubst_tm shift id (up_ty_ty tau_ty) (up_ty_tm tau_tm)
+            (funcomp (up_ty_ty tau_ty) shift) (funcomp (up_ty_tm tau_tm) id)
+            (fun x => eq_refl) (fun x => eq_refl) (sigma n))
+         (eq_trans
+            (eq_sym
+               (compSubstRen_tm tau_ty tau_tm shift id
+                  (funcomp (ren_ty shift) tau_ty)
+                  (funcomp (ren_tm shift id) tau_tm) (fun x => eq_refl)
+                  (fun x => eq_refl) (sigma n)))
+            (ap (ren_tm shift id) (Eq n)))).
 Qed.
 
 Lemma up_subst_subst_tm_ty (sigma : nat -> ty) (tau_ty : nat -> ty)
@@ -843,19 +838,15 @@ Lemma up_subst_subst_tm_ty (sigma : nat -> ty) (tau_ty : nat -> ty)
   (Eq : forall x, funcomp (subst_ty tau_ty) sigma x = theta x) :
   forall x,
   funcomp (subst_ty (up_tm_ty tau_ty)) (up_tm_ty sigma) x = up_tm_ty theta x.
-
 Proof.
 exact (fun n =>
-              eq_trans
-                (compRenSubst_ty id (up_tm_ty tau_ty)
-                   (funcomp (up_tm_ty tau_ty) id) (fun x => eq_refl)
-                   (sigma n))
-                (eq_trans
-                   (eq_sym
-                      (compSubstRen_ty tau_ty id (funcomp (ren_ty id) tau_ty)
-                         (fun x => eq_refl) (sigma n)))
-                   (ap (ren_ty id) (Eq n)))).
-
+       eq_trans
+         (compRenSubst_ty id (up_tm_ty tau_ty) (funcomp (up_tm_ty tau_ty) id)
+            (fun x => eq_refl) (sigma n))
+         (eq_trans
+            (eq_sym
+               (compSubstRen_ty tau_ty id (funcomp (ren_ty id) tau_ty)
+                  (fun x => eq_refl) (sigma n))) (ap (ren_ty id) (Eq n)))).
 Qed.
 
 Lemma up_subst_subst_tm_tm (sigma : nat -> tm) (tau_ty : nat -> ty)
@@ -864,26 +855,24 @@ Lemma up_subst_subst_tm_tm (sigma : nat -> tm) (tau_ty : nat -> ty)
   forall x,
   funcomp (subst_tm (up_tm_ty tau_ty) (up_tm_tm tau_tm)) (up_tm_tm sigma) x =
   up_tm_tm theta x.
-
 Proof.
 exact (fun n =>
-              match n with
-              | S n' =>
-                  eq_trans
-                    (compRenSubst_tm id shift (up_tm_ty tau_ty)
-                       (up_tm_tm tau_tm) (funcomp (up_tm_ty tau_ty) id)
-                       (funcomp (up_tm_tm tau_tm) shift) (fun x => eq_refl)
-                       (fun x => eq_refl) (sigma n'))
-                    (eq_trans
-                       (eq_sym
-                          (compSubstRen_tm tau_ty tau_tm id shift
-                             (funcomp (ren_ty id) tau_ty)
-                             (funcomp (ren_tm id shift) tau_tm)
-                             (fun x => eq_refl) (fun x => eq_refl) (sigma n')))
-                       (ap (ren_tm id shift) (Eq n')))
-              | O => eq_refl
-              end).
-
+       match n with
+       | S n' =>
+           eq_trans
+             (compRenSubst_tm id shift (up_tm_ty tau_ty) (up_tm_tm tau_tm)
+                (funcomp (up_tm_ty tau_ty) id)
+                (funcomp (up_tm_tm tau_tm) shift) (fun x => eq_refl)
+                (fun x => eq_refl) (sigma n'))
+             (eq_trans
+                (eq_sym
+                   (compSubstRen_tm tau_ty tau_tm id shift
+                      (funcomp (ren_ty id) tau_ty)
+                      (funcomp (ren_tm id shift) tau_tm) (fun x => eq_refl)
+                      (fun x => eq_refl) (sigma n')))
+                (ap (ren_tm id shift) (Eq n')))
+       | O => eq_refl
+       end).
 Qed.
 
 Fixpoint compSubstSubst_tm (sigma_ty : nat -> ty) (sigma_tm : nat -> tm)
@@ -922,41 +911,35 @@ subst_tm theta_ty theta_tm s :=
   end.
 
 Lemma rinstInst_up_ty_tm (xi : nat -> nat) (sigma : nat -> tm)
-  (Eq : forall x, funcomp var_tm xi x = sigma x) :
-  forall x, funcomp var_tm (upRen_ty_tm xi) x = up_ty_tm sigma x.
-
+  (Eq : forall x, funcomp (var_tm) xi x = sigma x) :
+  forall x, funcomp (var_tm) (upRen_ty_tm xi) x = up_ty_tm sigma x.
 Proof.
 exact (fun n => ap (ren_tm shift id) (Eq n)).
-
 Qed.
 
 Lemma rinstInst_up_tm_ty (xi : nat -> nat) (sigma : nat -> ty)
-  (Eq : forall x, funcomp var_ty xi x = sigma x) :
-  forall x, funcomp var_ty (upRen_tm_ty xi) x = up_tm_ty sigma x.
-
+  (Eq : forall x, funcomp (var_ty) xi x = sigma x) :
+  forall x, funcomp (var_ty) (upRen_tm_ty xi) x = up_tm_ty sigma x.
 Proof.
 exact (fun n => ap (ren_ty id) (Eq n)).
-
 Qed.
 
 Lemma rinstInst_up_tm_tm (xi : nat -> nat) (sigma : nat -> tm)
-  (Eq : forall x, funcomp var_tm xi x = sigma x) :
-  forall x, funcomp var_tm (upRen_tm_tm xi) x = up_tm_tm sigma x.
-
+  (Eq : forall x, funcomp (var_tm) xi x = sigma x) :
+  forall x, funcomp (var_tm) (upRen_tm_tm xi) x = up_tm_tm sigma x.
 Proof.
 exact (fun n =>
-              match n with
-              | S n' => ap (ren_tm id shift) (Eq n')
-              | O => eq_refl
-              end).
-
+       match n with
+       | S n' => ap (ren_tm id shift) (Eq n')
+       | O => eq_refl
+       end).
 Qed.
 
 Fixpoint rinst_inst_tm (xi_ty : nat -> nat) (xi_tm : nat -> nat)
 (sigma_ty : nat -> ty) (sigma_tm : nat -> tm)
-(Eq_ty : forall x, funcomp var_ty xi_ty x = sigma_ty x)
-(Eq_tm : forall x, funcomp var_tm xi_tm x = sigma_tm x) (s : tm) {struct s} :
-ren_tm xi_ty xi_tm s = subst_tm sigma_ty sigma_tm s :=
+(Eq_ty : forall x, funcomp (var_ty) xi_ty x = sigma_ty x)
+(Eq_tm : forall x, funcomp (var_tm) xi_tm x = sigma_tm x) (s : tm) {struct s}
+   : ren_tm xi_ty xi_tm s = subst_tm sigma_ty sigma_tm s :=
   match s with
   | var_tm s0 => Eq_tm s0
   | app s0 s1 =>
@@ -981,44 +964,573 @@ Lemma renRen_tm (xi_ty : nat -> nat) (xi_tm : nat -> nat)
   (zeta_ty : nat -> nat) (zeta_tm : nat -> nat) (s : tm) :
   ren_tm zeta_ty zeta_tm (ren_tm xi_ty xi_tm s) =
   ren_tm (funcomp zeta_ty xi_ty) (funcomp zeta_tm xi_tm) s.
-
 Proof.
-exact (compRenRen_tm xi_ty xi_tm zeta_ty zeta_tm _ _
-                (fun n => eq_refl) (fun n => eq_refl) s).
-
+exact (compRenRen_tm xi_ty xi_tm zeta_ty zeta_tm _ _ (fun n => eq_refl)
+         (fun n => eq_refl) s).
 Qed.
 
-Lemma compRen_tm (sigma_ty : nat -> ty) (sigma_tm : nat -> tm)
+Lemma renRen'_tm_pointwise (xi_ty : nat -> nat) (xi_tm : nat -> nat)
+  (zeta_ty : nat -> nat) (zeta_tm : nat -> nat) :
+  pointwise_relation _ eq
+    (funcomp (ren_tm zeta_ty zeta_tm) (ren_tm xi_ty xi_tm))
+    (ren_tm (funcomp zeta_ty xi_ty) (funcomp zeta_tm xi_tm)).
+Proof.
+exact (fun s =>
+       compRenRen_tm xi_ty xi_tm zeta_ty zeta_tm _ _ (fun n => eq_refl)
+         (fun n => eq_refl) s).
+Qed.
+
+Lemma substRen_tm (sigma_ty : nat -> ty) (sigma_tm : nat -> tm)
   (zeta_ty : nat -> nat) (zeta_tm : nat -> nat) (s : tm) :
   ren_tm zeta_ty zeta_tm (subst_tm sigma_ty sigma_tm s) =
   subst_tm (funcomp (ren_ty zeta_ty) sigma_ty)
     (funcomp (ren_tm zeta_ty zeta_tm) sigma_tm) s.
-
 Proof.
 exact (compSubstRen_tm sigma_ty sigma_tm zeta_ty zeta_tm _ _
-                (fun n => eq_refl) (fun n => eq_refl) s).
-
+         (fun n => eq_refl) (fun n => eq_refl) s).
 Qed.
 
-Lemma renComp_tm (xi_ty : nat -> nat) (xi_tm : nat -> nat)
+Lemma substRen_tm_pointwise (sigma_ty : nat -> ty) (sigma_tm : nat -> tm)
+  (zeta_ty : nat -> nat) (zeta_tm : nat -> nat) :
+  pointwise_relation _ eq
+    (funcomp (ren_tm zeta_ty zeta_tm) (subst_tm sigma_ty sigma_tm))
+    (subst_tm (funcomp (ren_ty zeta_ty) sigma_ty)
+       (funcomp (ren_tm zeta_ty zeta_tm) sigma_tm)).
+Proof.
+exact (fun s =>
+       compSubstRen_tm sigma_ty sigma_tm zeta_ty zeta_tm _ _
+         (fun n => eq_refl) (fun n => eq_refl) s).
+Qed.
+
+Lemma renSubst_tm (xi_ty : nat -> nat) (xi_tm : nat -> nat)
   (tau_ty : nat -> ty) (tau_tm : nat -> tm) (s : tm) :
   subst_tm tau_ty tau_tm (ren_tm xi_ty xi_tm s) =
   subst_tm (funcomp tau_ty xi_ty) (funcomp tau_tm xi_tm) s.
-
 Proof.
-exact (compRenSubst_tm xi_ty xi_tm tau_ty tau_tm _ _
-                (fun n => eq_refl) (fun n => eq_refl) s).
-
+exact (compRenSubst_tm xi_ty xi_tm tau_ty tau_tm _ _ (fun n => eq_refl)
+         (fun n => eq_refl) s).
 Qed.
 
-Lemma compComp_tm (sigma_ty : nat -> ty) (sigma_tm : nat -> tm)
+Lemma renSubst_tm_pointwise (xi_ty : nat -> nat) (xi_tm : nat -> nat)
+  (tau_ty : nat -> ty) (tau_tm : nat -> tm) :
+  pointwise_relation _ eq
+    (funcomp (subst_tm tau_ty tau_tm) (ren_tm xi_ty xi_tm))
+    (subst_tm (funcomp tau_ty xi_ty) (funcomp tau_tm xi_tm)).
+Proof.
+exact (fun s =>
+       compRenSubst_tm xi_ty xi_tm tau_ty tau_tm _ _ (fun n => eq_refl)
+         (fun n => eq_refl) s).
+Qed.
+
+Lemma substSubst_tm (sigma_ty : nat -> ty) (sigma_tm : nat -> tm)
   (tau_ty : nat -> ty) (tau_tm : nat -> tm) (s : tm) :
   subst_tm tau_ty tau_tm (subst_tm sigma_ty sigma_tm s) =
   subst_tm (funcomp (subst_ty tau_ty) sigma_ty)
     (funcomp (subst_tm tau_ty tau_tm) sigma_tm) s.
-
 Proof.
 exact (compSubstSubst_tm sigma_ty sigma_tm tau_ty tau_tm _ _
-                (fun n => eq_refl) (fun n => eq_refl) s).
-
+         (fun n => eq_refl) (fun n => eq_refl) s).
 Qed.
+
+Lemma substSubst_tm_pointwise (sigma_ty : nat -> ty) (sigma_tm : nat -> tm)
+  (tau_ty : nat -> ty) (tau_tm : nat -> tm) :
+  pointwise_relation _ eq
+    (funcomp (subst_tm tau_ty tau_tm) (subst_tm sigma_ty sigma_tm))
+    (subst_tm (funcomp (subst_ty tau_ty) sigma_ty)
+       (funcomp (subst_tm tau_ty tau_tm) sigma_tm)).
+Proof.
+exact (fun s =>
+       compSubstSubst_tm sigma_ty sigma_tm tau_ty tau_tm _ _
+         (fun n => eq_refl) (fun n => eq_refl) s).
+Qed.
+
+Lemma rinstInst'_tm (xi_ty : nat -> nat) (xi_tm : nat -> nat) (s : tm) :
+  ren_tm xi_ty xi_tm s =
+  subst_tm (funcomp (var_ty) xi_ty) (funcomp (var_tm) xi_tm) s.
+Proof.
+exact (rinst_inst_tm xi_ty xi_tm _ _ (fun n => eq_refl) (fun n => eq_refl) s).
+Qed.
+
+Lemma rinstInst'_tm_pointwise (xi_ty : nat -> nat) (xi_tm : nat -> nat) :
+  pointwise_relation _ eq (ren_tm xi_ty xi_tm)
+    (subst_tm (funcomp (var_ty) xi_ty) (funcomp (var_tm) xi_tm)).
+Proof.
+exact (fun s =>
+       rinst_inst_tm xi_ty xi_tm _ _ (fun n => eq_refl) (fun n => eq_refl) s).
+Qed.
+
+Lemma instId'_tm (s : tm) : subst_tm (var_ty) (var_tm) s = s.
+Proof.
+exact (idSubst_tm (var_ty) (var_tm) (fun n => eq_refl) (fun n => eq_refl) s).
+Qed.
+
+Lemma instId'_tm_pointwise :
+  pointwise_relation _ eq (subst_tm (var_ty) (var_tm)) id.
+Proof.
+exact (fun s =>
+       idSubst_tm (var_ty) (var_tm) (fun n => eq_refl) (fun n => eq_refl) s).
+Qed.
+
+Lemma rinstId'_tm (s : tm) : ren_tm id id s = s.
+Proof.
+exact (eq_ind_r (fun t => t = s) (instId'_tm s) (rinstInst'_tm id id s)).
+Qed.
+
+Lemma rinstId'_tm_pointwise : pointwise_relation _ eq (@ren_tm id id) id.
+Proof.
+exact (fun s =>
+       eq_ind_r (fun t => t = s) (instId'_tm s) (rinstInst'_tm id id s)).
+Qed.
+
+Lemma varL'_tm (sigma_ty : nat -> ty) (sigma_tm : nat -> tm) (x : nat) :
+  subst_tm sigma_ty sigma_tm (var_tm x) = sigma_tm x.
+Proof.
+exact (eq_refl).
+Qed.
+
+Lemma varL'_tm_pointwise (sigma_ty : nat -> ty) (sigma_tm : nat -> tm) :
+  pointwise_relation _ eq (funcomp (subst_tm sigma_ty sigma_tm) (var_tm))
+    sigma_tm.
+Proof.
+exact (fun x => eq_refl).
+Qed.
+
+Lemma varLRen'_tm (xi_ty : nat -> nat) (xi_tm : nat -> nat) (x : nat) :
+  ren_tm xi_ty xi_tm (var_tm x) = var_tm (xi_tm x).
+Proof.
+exact (eq_refl).
+Qed.
+
+Lemma varLRen'_tm_pointwise (xi_ty : nat -> nat) (xi_tm : nat -> nat) :
+  pointwise_relation _ eq (funcomp (ren_tm xi_ty xi_tm) (var_tm))
+    (funcomp (var_tm) xi_tm).
+Proof.
+exact (fun x => eq_refl).
+Qed.
+
+Class Up_tm X Y :=
+    up_tm : X -> Y.
+
+Class Up_ty X Y :=
+    up_ty : X -> Y.
+
+Instance Subst_tm : (Subst2 _ _ _ _) := @subst_tm.
+
+Instance Up_tm_tm : (Up_tm _ _) := @up_tm_tm.
+
+Instance Up_tm_ty : (Up_ty _ _) := @up_tm_ty.
+
+Instance Up_ty_tm : (Up_tm _ _) := @up_ty_tm.
+
+Instance Ren_tm : (Ren2 _ _ _ _) := @ren_tm.
+
+Instance VarInstance_tm : (Var _ _) := @var_tm.
+
+Instance Subst_ty : (Subst1 _ _ _) := @subst_ty.
+
+Instance Up_ty_ty : (Up_ty _ _) := @up_ty_ty.
+
+Instance Ren_ty : (Ren1 _ _ _) := @ren_ty.
+
+Instance VarInstance_ty : (Var _ _) := @var_ty.
+
+Notation "[ sigma_ty ; sigma_tm ]" := (subst_tm sigma_ty sigma_tm)
+  ( at level 1, left associativity, only printing) : fscope.
+
+Notation "s [ sigma_ty ; sigma_tm ]" := (subst_tm sigma_ty sigma_tm s)
+  ( at level 7, left associativity, only printing) : subst_scope.
+
+Notation "↑__tm" := up_tm (only printing) : subst_scope.
+
+Notation "↑__tm" := up_tm_tm (only printing) : subst_scope.
+
+Notation "↑__ty" := up_tm_ty (only printing) : subst_scope.
+
+Notation "↑__tm" := up_ty_tm (only printing) : subst_scope.
+
+Notation "⟨ xi_ty ; xi_tm ⟩" := (ren_tm xi_ty xi_tm)
+  ( at level 1, left associativity, only printing) : fscope.
+
+Notation "s ⟨ xi_ty ; xi_tm ⟩" := (ren_tm xi_ty xi_tm s)
+  ( at level 7, left associativity, only printing) : subst_scope.
+
+Notation "'var'" := var_tm ( at level 1, only printing) : subst_scope.
+
+Notation "x '__tm'" := (@ids _ _ VarInstance_tm x)
+  ( at level 5, format "x __tm", only printing) : subst_scope.
+
+Notation "x '__tm'" := (var_tm x) ( at level 5, format "x __tm") :
+  subst_scope.
+
+Notation "[ sigma_ty ]" := (subst_ty sigma_ty)
+  ( at level 1, left associativity, only printing) : fscope.
+
+Notation "s [ sigma_ty ]" := (subst_ty sigma_ty s)
+  ( at level 7, left associativity, only printing) : subst_scope.
+
+Notation "↑__ty" := up_ty (only printing) : subst_scope.
+
+Notation "↑__ty" := up_ty_ty (only printing) : subst_scope.
+
+Notation "⟨ xi_ty ⟩" := (ren_ty xi_ty)
+  ( at level 1, left associativity, only printing) : fscope.
+
+Notation "s ⟨ xi_ty ⟩" := (ren_ty xi_ty s)
+  ( at level 7, left associativity, only printing) : subst_scope.
+
+Notation "'var'" := var_ty ( at level 1, only printing) : subst_scope.
+
+Notation "x '__ty'" := (@ids _ _ VarInstance_ty x)
+  ( at level 5, format "x __ty", only printing) : subst_scope.
+
+Notation "x '__ty'" := (var_ty x) ( at level 5, format "x __ty") :
+  subst_scope.
+
+Instance subst_tm_morphism :
+ (Proper
+    (respectful (pointwise_relation _ eq)
+       (respectful (pointwise_relation _ eq) (respectful eq eq))) (@subst_tm)).
+Proof.
+exact (fun f_ty g_ty Eq_ty f_tm g_tm Eq_tm s t Eq_st =>
+       eq_ind s (fun t' => subst_tm f_ty f_tm s = subst_tm g_ty g_tm t')
+         (ext_tm f_ty f_tm g_ty g_tm Eq_ty Eq_tm s) t Eq_st).
+Qed.
+
+Instance ren_tm_morphism :
+ (Proper
+    (respectful (pointwise_relation _ eq)
+       (respectful (pointwise_relation _ eq) (respectful eq eq))) (@ren_tm)).
+Proof.
+exact (fun f_ty g_ty Eq_ty f_tm g_tm Eq_tm s t Eq_st =>
+       eq_ind s (fun t' => ren_tm f_ty f_tm s = ren_tm g_ty g_tm t')
+         (extRen_tm f_ty f_tm g_ty g_tm Eq_ty Eq_tm s) t Eq_st).
+Qed.
+
+Instance subst_ty_morphism :
+ (Proper (respectful (pointwise_relation _ eq) (respectful eq eq))
+    (@subst_ty)).
+Proof.
+exact (fun f_ty g_ty Eq_ty s t Eq_st =>
+       eq_ind s (fun t' => subst_ty f_ty s = subst_ty g_ty t')
+         (ext_ty f_ty g_ty Eq_ty s) t Eq_st).
+Qed.
+
+Instance ren_ty_morphism :
+ (Proper (respectful (pointwise_relation _ eq) (respectful eq eq)) (@ren_ty)).
+Proof.
+exact (fun f_ty g_ty Eq_ty s t Eq_st =>
+       eq_ind s (fun t' => ren_ty f_ty s = ren_ty g_ty t')
+         (extRen_ty f_ty g_ty Eq_ty s) t Eq_st).
+Qed.
+
+Ltac auto_unfold := repeat
+                     unfold VarInstance_ty, Var, ids, Ren_ty, Ren1, ren1,
+                      Up_ty_ty, Up_ty, up_ty, Subst_ty, Subst1, subst1,
+                      VarInstance_tm, Var, ids, Ren_tm, Ren2, ren2, Up_ty_tm,
+                      Up_tm, up_tm, Up_tm_ty, Up_ty, up_ty, Up_tm_tm, Up_tm,
+                      up_tm, Subst_tm, Subst2, subst2.
+
+Tactic Notation "auto_unfold" "in" "*" := repeat
+                                           unfold VarInstance_ty, Var, ids,
+                                            Ren_ty, Ren1, ren1, Up_ty_ty,
+                                            Up_ty, up_ty, Subst_ty, Subst1,
+                                            subst1, VarInstance_tm, Var, ids,
+                                            Ren_tm, Ren2, ren2, Up_ty_tm,
+                                            Up_tm, up_tm, Up_tm_ty, Up_ty,
+                                            up_ty, Up_tm_tm, Up_tm, up_tm,
+                                            Subst_tm, Subst2, subst2 
+                                            in *.
+
+Ltac asimpl' := repeat (first
+                 [ progress setoid_rewrite substSubst_tm_pointwise
+                 | progress setoid_rewrite substSubst_tm
+                 | progress setoid_rewrite renSubst_tm_pointwise
+                 | progress setoid_rewrite renSubst_tm
+                 | progress setoid_rewrite substRen_tm_pointwise
+                 | progress setoid_rewrite substRen_tm
+                 | progress setoid_rewrite renRen'_tm_pointwise
+                 | progress setoid_rewrite renRen_tm
+                 | progress setoid_rewrite substSubst_ty_pointwise
+                 | progress setoid_rewrite substSubst_ty
+                 | progress setoid_rewrite renSubst_ty_pointwise
+                 | progress setoid_rewrite renSubst_ty
+                 | progress setoid_rewrite substRen_ty_pointwise
+                 | progress setoid_rewrite substRen_ty
+                 | progress setoid_rewrite renRen'_ty_pointwise
+                 | progress setoid_rewrite renRen_ty
+                 | progress setoid_rewrite varLRen'_tm_pointwise
+                 | progress setoid_rewrite varLRen'_tm
+                 | progress setoid_rewrite varL'_tm_pointwise
+                 | progress setoid_rewrite varL'_tm
+                 | progress setoid_rewrite rinstId'_tm_pointwise
+                 | progress setoid_rewrite rinstId'_tm
+                 | progress setoid_rewrite instId'_tm_pointwise
+                 | progress setoid_rewrite instId'_tm
+                 | progress setoid_rewrite varLRen'_ty_pointwise
+                 | progress setoid_rewrite varLRen'_ty
+                 | progress setoid_rewrite varL'_ty_pointwise
+                 | progress setoid_rewrite varL'_ty
+                 | progress setoid_rewrite rinstId'_ty_pointwise
+                 | progress setoid_rewrite rinstId'_ty
+                 | progress setoid_rewrite instId'_ty_pointwise
+                 | progress setoid_rewrite instId'_ty
+                 | progress
+                    unfold up_tm_tm, up_tm_ty, up_ty_tm, upRen_tm_tm,
+                     upRen_tm_ty, upRen_ty_tm, up_ty_ty, upRen_ty_ty, up_ren
+                 | progress cbn[subst_tm ren_tm subst_ty ren_ty]
+                 | progress fsimpl ]).
+
+Ltac asimpl := check_no_evars;
+                repeat
+                 unfold VarInstance_ty, Var, ids, Ren_ty, Ren1, ren1,
+                  Up_ty_ty, Up_ty, up_ty, Subst_ty, Subst1, subst1,
+                  VarInstance_tm, Var, ids, Ren_tm, Ren2, ren2, Up_ty_tm,
+                  Up_tm, up_tm, Up_tm_ty, Up_ty, up_ty, Up_tm_tm, Up_tm,
+                  up_tm, Subst_tm, Subst2, subst2 in *; asimpl'; minimize.
+
+Tactic Notation "asimpl" "in" hyp(J) := revert J; asimpl; intros J.
+
+Tactic Notation "auto_case" := auto_case ltac:(asimpl; cbn; eauto).
+
+Ltac substify := auto_unfold; try setoid_rewrite rinstInst'_tm_pointwise;
+                  try setoid_rewrite rinstInst'_tm;
+                  try setoid_rewrite rinstInst'_ty_pointwise;
+                  try setoid_rewrite rinstInst'_ty.
+
+Ltac renamify := auto_unfold; try setoid_rewrite_left rinstInst'_tm_pointwise;
+                  try setoid_rewrite_left rinstInst'_tm;
+                  try setoid_rewrite_left rinstInst'_ty_pointwise;
+                  try setoid_rewrite_left rinstInst'_ty.
+
+End Core.
+
+Module Fext.
+
+Import
+Core.
+
+Lemma rinstInst_ty (xi_ty : nat -> nat) :
+  ren_ty xi_ty = subst_ty (funcomp (var_ty) xi_ty).
+Proof.
+exact (FunctionalExtensionality.functional_extensionality _ _
+         (fun x => rinst_inst_ty xi_ty _ (fun n => eq_refl) x)).
+Qed.
+
+Lemma instId_ty : subst_ty (var_ty) = id.
+Proof.
+exact (FunctionalExtensionality.functional_extensionality _ _
+         (fun x => idSubst_ty (var_ty) (fun n => eq_refl) (id x))).
+Qed.
+
+Lemma rinstId_ty : @ren_ty id = id.
+Proof.
+exact (eq_trans (rinstInst_ty (id _)) instId_ty).
+Qed.
+
+Lemma varL_ty (sigma_ty : nat -> ty) :
+  funcomp (subst_ty sigma_ty) (var_ty) = sigma_ty.
+Proof.
+exact (FunctionalExtensionality.functional_extensionality _ _
+         (fun x => eq_refl)).
+Qed.
+
+Lemma varLRen_ty (xi_ty : nat -> nat) :
+  funcomp (ren_ty xi_ty) (var_ty) = funcomp (var_ty) xi_ty.
+Proof.
+exact (FunctionalExtensionality.functional_extensionality _ _
+         (fun x => eq_refl)).
+Qed.
+
+Lemma renRen'_ty (xi_ty : nat -> nat) (zeta_ty : nat -> nat) :
+  funcomp (ren_ty zeta_ty) (ren_ty xi_ty) = ren_ty (funcomp zeta_ty xi_ty).
+Proof.
+exact (FunctionalExtensionality.functional_extensionality _ _
+         (fun n => renRen_ty xi_ty zeta_ty n)).
+Qed.
+
+Lemma substRen'_ty (sigma_ty : nat -> ty) (zeta_ty : nat -> nat) :
+  funcomp (ren_ty zeta_ty) (subst_ty sigma_ty) =
+  subst_ty (funcomp (ren_ty zeta_ty) sigma_ty).
+Proof.
+exact (FunctionalExtensionality.functional_extensionality _ _
+         (fun n => substRen_ty sigma_ty zeta_ty n)).
+Qed.
+
+Lemma renSubst'_ty (xi_ty : nat -> nat) (tau_ty : nat -> ty) :
+  funcomp (subst_ty tau_ty) (ren_ty xi_ty) = subst_ty (funcomp tau_ty xi_ty).
+Proof.
+exact (FunctionalExtensionality.functional_extensionality _ _
+         (fun n => renSubst_ty xi_ty tau_ty n)).
+Qed.
+
+Lemma substSubst'_ty (sigma_ty : nat -> ty) (tau_ty : nat -> ty) :
+  funcomp (subst_ty tau_ty) (subst_ty sigma_ty) =
+  subst_ty (funcomp (subst_ty tau_ty) sigma_ty).
+Proof.
+exact (FunctionalExtensionality.functional_extensionality _ _
+         (fun n => substSubst_ty sigma_ty tau_ty n)).
+Qed.
+
+Lemma rinstInst_tm (xi_ty : nat -> nat) (xi_tm : nat -> nat) :
+  ren_tm xi_ty xi_tm =
+  subst_tm (funcomp (var_ty) xi_ty) (funcomp (var_tm) xi_tm).
+Proof.
+exact (FunctionalExtensionality.functional_extensionality _ _
+         (fun x =>
+          rinst_inst_tm xi_ty xi_tm _ _ (fun n => eq_refl) (fun n => eq_refl)
+            x)).
+Qed.
+
+Lemma instId_tm : subst_tm (var_ty) (var_tm) = id.
+Proof.
+exact (FunctionalExtensionality.functional_extensionality _ _
+         (fun x =>
+          idSubst_tm (var_ty) (var_tm) (fun n => eq_refl) (fun n => eq_refl)
+            (id x))).
+Qed.
+
+Lemma rinstId_tm : @ren_tm id id = id.
+Proof.
+exact (eq_trans (rinstInst_tm (id _) (id _)) instId_tm).
+Qed.
+
+Lemma varL_tm (sigma_ty : nat -> ty) (sigma_tm : nat -> tm) :
+  funcomp (subst_tm sigma_ty sigma_tm) (var_tm) = sigma_tm.
+Proof.
+exact (FunctionalExtensionality.functional_extensionality _ _
+         (fun x => eq_refl)).
+Qed.
+
+Lemma varLRen_tm (xi_ty : nat -> nat) (xi_tm : nat -> nat) :
+  funcomp (ren_tm xi_ty xi_tm) (var_tm) = funcomp (var_tm) xi_tm.
+Proof.
+exact (FunctionalExtensionality.functional_extensionality _ _
+         (fun x => eq_refl)).
+Qed.
+
+Lemma renRen'_tm (xi_ty : nat -> nat) (xi_tm : nat -> nat)
+  (zeta_ty : nat -> nat) (zeta_tm : nat -> nat) :
+  funcomp (ren_tm zeta_ty zeta_tm) (ren_tm xi_ty xi_tm) =
+  ren_tm (funcomp zeta_ty xi_ty) (funcomp zeta_tm xi_tm).
+Proof.
+exact (FunctionalExtensionality.functional_extensionality _ _
+         (fun n => renRen_tm xi_ty xi_tm zeta_ty zeta_tm n)).
+Qed.
+
+Lemma substRen'_tm (sigma_ty : nat -> ty) (sigma_tm : nat -> tm)
+  (zeta_ty : nat -> nat) (zeta_tm : nat -> nat) :
+  funcomp (ren_tm zeta_ty zeta_tm) (subst_tm sigma_ty sigma_tm) =
+  subst_tm (funcomp (ren_ty zeta_ty) sigma_ty)
+    (funcomp (ren_tm zeta_ty zeta_tm) sigma_tm).
+Proof.
+exact (FunctionalExtensionality.functional_extensionality _ _
+         (fun n => substRen_tm sigma_ty sigma_tm zeta_ty zeta_tm n)).
+Qed.
+
+Lemma renSubst'_tm (xi_ty : nat -> nat) (xi_tm : nat -> nat)
+  (tau_ty : nat -> ty) (tau_tm : nat -> tm) :
+  funcomp (subst_tm tau_ty tau_tm) (ren_tm xi_ty xi_tm) =
+  subst_tm (funcomp tau_ty xi_ty) (funcomp tau_tm xi_tm).
+Proof.
+exact (FunctionalExtensionality.functional_extensionality _ _
+         (fun n => renSubst_tm xi_ty xi_tm tau_ty tau_tm n)).
+Qed.
+
+Lemma substSubst'_tm (sigma_ty : nat -> ty) (sigma_tm : nat -> tm)
+  (tau_ty : nat -> ty) (tau_tm : nat -> tm) :
+  funcomp (subst_tm tau_ty tau_tm) (subst_tm sigma_ty sigma_tm) =
+  subst_tm (funcomp (subst_ty tau_ty) sigma_ty)
+    (funcomp (subst_tm tau_ty tau_tm) sigma_tm).
+Proof.
+exact (FunctionalExtensionality.functional_extensionality _ _
+         (fun n => substSubst_tm sigma_ty sigma_tm tau_ty tau_tm n)).
+Qed.
+
+Ltac asimpl_fext' := repeat (first
+                      [ progress setoid_rewrite substSubst_tm_pointwise
+                      | progress setoid_rewrite substSubst_tm
+                      | progress setoid_rewrite renSubst_tm_pointwise
+                      | progress setoid_rewrite renSubst_tm
+                      | progress setoid_rewrite substRen_tm_pointwise
+                      | progress setoid_rewrite substRen_tm
+                      | progress setoid_rewrite renRen'_tm_pointwise
+                      | progress setoid_rewrite renRen_tm
+                      | progress setoid_rewrite substSubst_ty_pointwise
+                      | progress setoid_rewrite substSubst_ty
+                      | progress setoid_rewrite renSubst_ty_pointwise
+                      | progress setoid_rewrite renSubst_ty
+                      | progress setoid_rewrite substRen_ty_pointwise
+                      | progress setoid_rewrite substRen_ty
+                      | progress setoid_rewrite renRen'_ty_pointwise
+                      | progress setoid_rewrite renRen_ty
+                      | progress setoid_rewrite substSubst'_tm
+                      | progress setoid_rewrite renSubst'_tm
+                      | progress setoid_rewrite substRen'_tm
+                      | progress setoid_rewrite renRen'_tm
+                      | progress setoid_rewrite varLRen_tm
+                      | progress setoid_rewrite varL_tm
+                      | progress setoid_rewrite rinstId_tm
+                      | progress setoid_rewrite instId_tm
+                      | progress setoid_rewrite substSubst'_ty
+                      | progress setoid_rewrite renSubst'_ty
+                      | progress setoid_rewrite substRen'_ty
+                      | progress setoid_rewrite renRen'_ty
+                      | progress setoid_rewrite varLRen_ty
+                      | progress setoid_rewrite varL_ty
+                      | progress setoid_rewrite rinstId_ty
+                      | progress setoid_rewrite instId_ty
+                      | progress
+                         unfold up_tm_tm, up_tm_ty, up_ty_tm, upRen_tm_tm,
+                          upRen_tm_ty, upRen_ty_tm, up_ty_ty, upRen_ty_ty,
+                          up_ren
+                      | progress cbn[subst_tm ren_tm subst_ty ren_ty]
+                      | fsimpl_fext ]).
+
+Ltac asimpl_fext := check_no_evars; repeat try unfold_funcomp;
+                     repeat
+                      unfold VarInstance_ty, Var, ids, Ren_ty, Ren1, ren1,
+                       Up_ty_ty, Up_ty, up_ty, Subst_ty, Subst1, subst1,
+                       VarInstance_tm, Var, ids, Ren_tm, Ren2, ren2,
+                       Up_ty_tm, Up_tm, up_tm, Up_tm_ty, Up_ty, up_ty,
+                       Up_tm_tm, Up_tm, up_tm, Subst_tm, Subst2, subst2 
+                       in *; asimpl_fext'; repeat try unfold_funcomp.
+
+Tactic Notation "asimpl_fext" "in" hyp(J) := revert J; asimpl_fext; intros J.
+
+Ltac substify_fext := auto_unfold; try repeat erewrite ?rinstInst_tm;
+                       try repeat erewrite ?rinstInst_ty.
+
+Ltac renamify_fext := auto_unfold; try repeat erewrite <- ?rinstInst_tm;
+                       try repeat erewrite <- ?rinstInst_ty.
+
+End Fext.
+
+Module Extra.
+
+Import Core.
+
+Import
+Core.
+
+Hint Opaque subst_tm: rewrite.
+
+Hint Opaque ren_tm: rewrite.
+
+Hint Opaque subst_ty: rewrite.
+
+Hint Opaque ren_ty: rewrite.
+
+End Extra.
+
+Module interface.
+
+Export Core.
+
+Export Fext.
+
+Export Extra.
+
+End interface.
+
+Export interface.
+
