case-studies/tapl-exercise/unscoped.v
@@ -30,6 +30,8 @@ Definition scons {X: Type} (x : X) (xi : nat -> X) :=
         | S n => xi n
         end.
 
+Hint Opaque scons : rewrite.
+
 (** ** Type Class Instances for Notation
 Required to make notation work. *)
 
@@ -105,7 +107,9 @@ Module CombineNotations.
 
   Notation "s .: sigma" := (scons s sigma) (at level 55, sigma at next level, right associativity) : subst_scope.
 
+  #[ global ]
   Open Scope fscope.
+  #[ global ]
   Open Scope subst_scope.
 End CombineNotations.
 
@@ -126,25 +130,33 @@ Proof.
 Qed.
 
 (** Eta laws. *)
-Lemma scons_eta' {T} (f : nat -> T) (x: nat) :
-  (f var_zero .: (fun x => f (shift x))) x = f x.
-Proof. destruct x; reflexivity. Qed.
+Lemma scons_eta' {T} (f : nat -> T) :
+  pointwise_relation _ eq (f var_zero .: (funcomp f shift)) f.
+Proof. intros x. destruct x; reflexivity. Qed.
 
-Lemma scons_eta_id' (x: nat) :
-  (var_zero .: shift) x = id x.
-Proof. destruct x; reflexivity. Qed.
+Lemma scons_eta_id' :
+  pointwise_relation _ eq (var_zero .: shift) id.
+Proof. intros x. destruct x; reflexivity. Qed.
 
-Lemma scons_comp' (T: Type) {U} (s: T) (sigma: nat -> T) (tau: T -> U ) (x: nat) :
-  tau ((s .: sigma) x) = ((tau s) .: (fun x => tau (sigma x))) x.
-Proof. destruct x; reflexivity. Qed.
+Lemma scons_comp' (T: Type) {U} (s: T) (sigma: nat -> T) (tau: T -> U) :
+  pointwise_relation _ eq (funcomp tau (s .: sigma)) ((tau s) .: (funcomp tau sigma)).
+Proof. intros x. destruct x; reflexivity. Qed.
 
 (* Morphism for Setoid Rewriting. The only morphism that can be defined statically. *)
-Instance scons_morphism {X: Type}:
+Instance scons_morphism {X: Type} :
   Proper (eq ==> pointwise_relation _ eq ==> pointwise_relation _ eq) (@scons X).
 Proof.
-  cbv - [scons].
-  intros t t' -> sigma tau H.
+  intros ? t -> sigma tau H.
   intros [|x].
+  cbn. reflexivity.
+  apply H.
+Qed.
+
+Instance scons_morphism2 {X: Type} :
+  Proper (eq ==> pointwise_relation _ eq ==> eq ==> eq) (@scons X).
+Proof.
+  intros ? t -> sigma tau H ? x ->.
+  destruct x as [|x].
   cbn. reflexivity.
   apply H.
 Qed.
@@ -172,11 +184,6 @@ End UnscopedNotations.
 
 (** ** Tactics for unscoped syntax *)
 
-Ltac unfold_funcomp := match goal with
-                       | |-  context[(?f >> ?g) ?s] => change ((f >> g) s) with (g (f s))
-                       end.
-
-
 (** Automatically does a case analysis on a natural number, useful for proofs with context renamings/context morphisms. *)
 Tactic Notation "auto_case" tactic(t) :=  (match goal with
                                            | [|- forall (i : nat), _] => intros []; t
@@ -185,22 +192,24 @@ Tactic Notation "auto_case" tactic(t) :=  (match goal with
 
 (** Generic fsimpl tactic: simplifies the above primitives in a goal. *)
 Ltac fsimpl :=
+  (* TODO why unfold upren *)
   unfold up_ren; repeat match goal with
          | [|- context[id >> ?f]] => change (id >> f) with f (* AsimplCompIdL *)
          | [|- context[?f >> id]] => change (f >> id) with f (* AsimplCompIdR *)
          | [|- context [id ?s]] => change (id s) with s
          | [|- context[(?f >> ?g) >> ?h]] => change ((f >> g) >> h) with (f >> (g >> h))
-         | [|- context[(?s .: ?sigma) var_zero]] => change ((s .: sigma) var_zero) with s
-         (* TODO check if below rule is not redundant *)
+         | [|- context[(?v .: ?g) var_zero]] => change ((v .: g) var_zero) with v
          | [|- context[(?v .: ?g) 0]] => change ((v .: g) 0) with v
          | [|- context[(?v .: ?g) (S ?n)]] => change ((v .: g) (S n)) with (g n)
          | [|- context[?f >> (?x .: ?g)]] => change (f >> (x .: g)) with g (* f should evaluate to shift *)
          | [|- context[var_zero]] =>  change var_zero with 0
-         | [|- context[?x2 .: (fun x => ?f (shift x))]] => change (scons x2 (fun x => f (shift x))) with (fun x => (scons (f var_zero) (fun x => f (shift x))) x); setoid_rewrite (@scons_eta' _ _ f)
-         | [|- context[?f var_zero .: ?g]] => change (scons (f var_zero) g) with (fun x => (scons (f var_zero) (fun x => f (shift x))) x); rewrite scons_eta'
-         (* TODO had to put an underscore as the last argument to scons. This might be an argument against unfolding funcomp *)
-         | [|- context[fun x => ?tau (scons ?s ?sigma _)]] => setoid_rewrite scons_comp'; eta_reduce
-         | [|- context[scons var_zero shift]] => change (scons var_zero shift) with (fun x => (scons var_zero shift) x); setoid_rewrite scons_eta_id'; eta_reduce
+         | [|- context[?x2 .: (funcomp ?f shift)]] => change (scons x2 (funcomp f shift)) with (scons (f var_zero) (funcomp f shift)); setoid_rewrite (@scons_eta' _ _ f)
+         | [|- context[?f var_zero .: ?g]] => change (scons (f var_zero) g) with (scons (f var_zero) (funcomp f shift)); rewrite scons_eta'
+         | [|- _ =  ?h (?f ?s)] => change (h (f s)) with ((f >> h) s)
+         | [|-  ?h (?f ?s) = _] => change (h (f s)) with ((f >> h) s)
+         (* DONE had to put an underscore as the last argument to scons. This might be an argument against unfolding funcomp *)
+         | [|- context[funcomp _ (scons _ _)]] => setoid_rewrite scons_comp'; eta_reduce
+         | [|- context[scons var_zero shift]] => setoid_rewrite scons_eta_id'; eta_reduce
                         end.
 
 (* TODO rewrite fsimplc. Leave for now because it's never used. *)
